Make case study specs more uniform.

examples/store/proofs/base.v
@@ -70,11 +70,20 @@ Implicit Types b : bool.
 Implicit Types v : val.
 Implicit Types (failed : bool).
 
-Definition db_client_ready skI skR db : iProp :=
-  rep_main skI skR dbN db ∗ rep_sync skI skR dbN ∅ db.
+Definition db_main skI skR db : iProp :=
+  rep_main skI skR dbN db.
 
-Definition db_server_ready skI skR db : iProp :=
+Definition db_sync skI skR db : iProp :=
+  rep_sync skI skR dbN ∅ db.
+
+Definition db_copy skI skR db : iProp :=
   rep_copy skI skR dbN ∅ db.
+
+Definition db_update skI skR db db' : iProp :=
+  rep_update skI skR dbN ∅ db db'.
+
+Definition db_client_ready skI skR db : iProp :=
+  db_main skI skR db ∗ db_sync skI skR db.
 
 Definition db_disconnected skI skR : iProp := ∃ db,
   (Conn.failure skI skR ∨ db_client_ready skI skR db) ∗
@@ -152,7 +161,7 @@ Qed.
 Definition server_db_connected' skI skR cs vdb : iProp := ∃ db,
   public_db db ∗
   AList.is_alist vdb (repr <$> db) ∗
-  (compromised Resp cs ∨ db_server_ready skI skR db).
+  (compromised Resp cs ∨ db_copy skI skR db).
 
 Definition server_db_connected skI skR cs vdb : iProp :=
   RPC.server_connected skI skR cs ∗
@@ -164,7 +173,7 @@ Definition server_handler skI skR cs vdb h : iProp :=
 Definition server_db_disconnected skI skR vdb : iProp := ∃ db,
   public_db db ∗
   AList.is_alist vdb (repr <$> db) ∗
-  (Conn.failure skI skR ∨ db_server_ready skI skR db).
+  (Conn.failure skI skR ∨ db_copy skI skR db).
 
 Lemma server_db_alloc skI skR vdb E :
   ↑dbN.@"server".@(skI : term) ⊆ E →
@@ -203,10 +212,10 @@ Qed.
 Definition store_call_pred skI skR si ts : iProp :=
   ∃ t1 t2 db,
     ⌜ts = [t1; t2]⌝ ∗
-    rep_update skI skR dbN ∅ db (<[t1 := t2]> db).
+    db_update skI skR db (<[t1 := t2]> db).
 
 Definition store_resp_pred skI skR si ts ts' : iProp :=
-  ∃ db, rep_sync skI skR dbN ∅ db.
+  ∃ db, db_sync skI skR db.
 
 Lemma store_call t2' skI skR cs t1 t2 :
   let P := compromised Init cs in
@@ -235,9 +244,9 @@ Qed.
 
 Lemma store_resp skI skR cs db t1 t2 :
   let P := compromised Resp cs in
-  (P ∨ db_server_ready skI skR db) -∗
+  (P ∨ db_copy skI skR db) -∗
   (P ∨ store_call_pred skI skR cs [t1; t2]) ==∗
-  (P ∨ db_server_ready skI skR (<[t1 := t2]>db)) ∗
+  (P ∨ db_copy skI skR (<[t1 := t2]>db)) ∗
   (P ∨ store_resp_pred skI skR cs [t1; t2] [TInt 0]).
 Proof.
 iIntros "% [#?|ready] [#?|call]"; try by iModIntro; iSplitL; eauto.
@@ -249,10 +258,10 @@ Qed.
 
 Definition create_call_pred skI skR si ts : iProp :=
   ∃ t1 t2 db, ⌜ts = [t1; t2]⌝ ∗ ⌜db !! t1 = None⌝ ∗
-    rep_update skI skR dbN ∅ db (<[t1 := t2]>db).
+    db_update skI skR db (<[t1 := t2]>db).
 
 Definition create_resp_pred skI skR si ts ts' : iProp :=
-  ∃ db, rep_sync skI skR dbN ∅ db.
+  ∃ db, db_sync skI skR db.
 
 Lemma create_call t1 t2 skI skR cs :
   let P := compromised Init cs in
@@ -281,9 +290,9 @@ Qed.
 
 Lemma create_resp skI skR cs db t1 t2 :
   let P := compromised Resp cs in
-  (P ∨ db_server_ready skI skR db) -∗
+  (P ∨ db_copy skI skR db) -∗
   (P ∨ create_call_pred skI skR cs [t1; t2]) ==∗
-  (P ∨ db_server_ready skI skR (<[t1 := t2]>db)) ∗
+  (P ∨ db_copy skI skR (<[t1 := t2]>db)) ∗
   (P ∨ create_resp_pred skI skR cs [t1; t2] [TInt 0]).
 Proof.
 iIntros "% [#?|ready] [#?|call]"; try by iModIntro; iSplitL; eauto.
@@ -295,11 +304,11 @@ Qed.
 
 Definition load_call_pred skI skR si ts : iProp :=
   ∃ t1 t2 db, ⌜ts = [t1]⌝ ∗ ⌜db !! t1 = Some t2⌝ ∗
-              rep_update skI skR dbN ∅ db db.
+              db_update skI skR db db.
 
 Definition load_resp_pred skI skR si ts ts' : iProp :=
   ∃ t1 t2 db, ⌜ts = [t1]⌝ ∗ ⌜ts' = [t2]⌝ ∗ ⌜db !! t1 = Some t2⌝ ∗
-              rep_sync skI skR dbN ∅ db.
+              db_sync skI skR db.
 
 Lemma load_call t1 t2 skI skR cs :
   let P := compromised Init cs in
@@ -331,9 +340,9 @@ Qed.
 Lemma load_resp skI skR cs db t1 :
   let P := compromised Resp cs in
   let t2 := default (TInt 0) (db !! t1) in
-  (P ∨ db_server_ready skI skR db) -∗
+  (P ∨ db_copy skI skR db) -∗
   (P ∨ load_call_pred skI skR cs [t1]) ==∗
-  (P ∨ db_server_ready skI skR db) ∗
+  (P ∨ db_copy skI skR db) ∗
   (P ∨ load_resp_pred skI skR cs [t1] [t2]).
 Proof.
 iIntros "%P /= [#?|ready] [#?|call]"; try by iModIntro; iSplitL; eauto.
