examples/store/proofs/client/store.v
@@ -27,21 +27,21 @@ Implicit Types γ : gname.
 Implicit Types v : val.
 
 Lemma wp_client_store skI skR cs t1 t2 t2' :
-  cryptis_ctx -∗
-  store_ctx -∗
-  public t1 -∗
+  cryptis_ctx ∗
+  store_ctx ∗
+  public t1 ∗
   public t2' -∗
   {{{ db_connected skI skR cs ∗ db_mapsto skI skR t1 t2 }}}
     Client.store (repr cs) t1 t2'
   {{{ RET #(); db_connected skI skR cs ∗ db_mapsto skI skR t1 t2' }}}.
 Proof.
-iIntros "#? #ctx #p_t1 #p_t2 !> %Φ [client mapsto] post".
+iIntros "(#? & #ctx & #p_t1 & #p_t2) !> %Φ [client mapsto] post".
 iDestruct "client" as "(conn & db)".
 iMod (store_call t2' with "db mapsto") as "(store & mapsto & waiting)".
 wp_lam. wp_pures. wp_list.
 iPoseProof (store_ctx_store with "[//]") as "?".
 iPoseProof (store_ctx_rpc_ctx with "[//]") as "?".
-wp_apply (RPC.wp_call with "[$conn $store]").
+wp_apply (RPC.wp_call with "[] [$conn $store]").
 { do 4!iSplit => //=; first by eauto. }
 iIntros "%ts' (conn & store & _)". wp_pures. iApply "post".
 iFrame. by iApply "waiting".
